ExistentialRules/ChaseSequence/ChaseDerivation.lean
@@ -284,195 +284,24 @@ end InductionPrinciple
 
 end Basics
 
-public section FactMonotonicity
-
-/-!
-## Subset Monotonicity of Facts in ChaseNodes
-
-Compared to `ChaseDerivationSkeleton`, we get a couple of nice implications out of the subset monotonicity of fact sets. For example, we can never see the same `ChaseNode` twice as otherwise the trigger in second occurrence would already be obsolete.
--/
-
-/-- Each member's facts contain the head facts. Note that this extends to arbitrary pairs of members since each member always induces a subderivation where it acts as the head. -/
-@[grind <-]
-theorem facts_node_subset_every_mem {cd : ChaseDerivation (RegularChaseNode obs rules) obs rules} : ∀ node ∈ cd, cd.head.facts ⊆ node.facts :=
-  ChaseDerivationSkeleton.facts_node_subset_every_mem
-
-/-- A first implication of `facts_node_subset_every_mem` is that, considering one of our subderivations, each of our members either has all of its facts contained in the head of the subderivation or it is itself a member of the subderivation. -/
-theorem mem_suffix_of_mem {cd1 cd2 : ChaseDerivation (RegularChaseNode obs rules) obs rules} (suffix : cd1 <:+ cd2) : ∀ node ∈ cd2, node.facts ⊆ cd1.head.facts ∨ node ∈ cd1 :=
-  ChaseDerivationSkeleton.mem_suffix_of_mem suffix
-
-/-- The `head` cannot occur in the `tail`. Otherwise, it would be introduced using a trigger but then this trigger is already obsolete since all the facts from `head` already occur in the very beginning. We use `ObsolescenceCondition.contains_trg_result_implies_cond` here. -/
-theorem head_not_mem_tail {cd : ChaseDerivation (RegularChaseNode obs rules) obs rules} : ∀ h, ¬ cd.head ∈ cd.tail h := by
-  intro h contra
-  rw [mem_tail_iff] at contra
-  rcases contra with ⟨cd2, suffix, contra⟩
-  apply (cd2.active_trigger_origin_next contra).right
-  apply obs.contains_trg_result_implies_cond
-  apply Set.subset_trans (cd.head.facts_contain_origin_result (cd.head.origin.get (cd2.isSome_origin_next contra)) (by simp))
-  apply cd.facts_node_subset_every_mem
-  apply mem_of_mem_suffix suffix
-  exact cd2.head_mem
-
-/-- By `head_not_mem_tail`, if we have a suffix but our head occurs in the suffix, then our suffix is equal to us. -/
-@[grind ->]
-theorem eq_of_suffix_of_head_mem {cd1 cd2 : ChaseDerivation (RegularChaseNode obs rules) obs rules} (suffix : cd1 <:+ cd2) (head_mem : cd2.head ∈ cd1) : cd1 = cd2 := by
-  rw [suffix_iff_eq_or_suffix_tail] at suffix
-  cases suffix with
-  | inl suffix => exact suffix
-  | inr suffix => rcases suffix with ⟨h, suffix⟩; apply False.elim; apply head_not_mem_tail h; apply mem_of_mem_suffix suffix; exact head_mem
-
-/-- And now by `eq_of_suffix_of_head_mem`, if we have two suffixes $C$ and $D$, and the head of $D$ occurs in $C$, then $D$ is a suffix of $C$. This may seem obvious even without the above results but it is really not even though it aligns well with one's intuition. Imagine that a `ChaseNode` could occur multiple times in a `ChaseDerivation`. Then we may have a case where $C$ is a subderivation of $D$, $D$ is not a subderivation of $C$ but $D$ occurs in $C$. -/
-@[grind ->]
-theorem suffix_of_suffix_of_suffix_of_head_mem {cd cd1 cd2 : ChaseDerivation (RegularChaseNode obs rules) obs rules} : cd1 <:+ cd -> cd2 <:+ cd -> cd2.head ∈ cd1 -> cd2 <:+ cd1 := by
-  intro suffix1 suffix2 head_mem
-  cases PossiblyInfiniteList.suffix_or_suffix_of_suffix suffix1 suffix2 with
-  | inr suffix => exact suffix
-  | inl suffix => rw [eq_of_suffix_of_head_mem suffix]; exact PossiblyInfiniteList.IsSuffix_refl; exact head_mem
-
-end FactMonotonicity
-
 public section Predecessors
 
 /-!
 ## Predecessor Relation
 
-Since we learned that `ChaseNode`s cannot occur multiple times in the same `ChaseDerivation`,
-the predecessor relation defined on `ChaseDerivationSkeleton` is now a total order on `ChaseDerivation.Node`.
-This is particularly nice, since we can do this while completely ignoring indices of the nodes in the underlying `PossiblyInfiniteList`.
+We lift the predecessor relation from `ChaseDerivationSkeleton`s to `ChaseDerivation`s.
 -/
 
+variable {N : Type u} [CN : ChaseNode N obs rules]
+
 /-- We could also define the predecessor relation directly on `ChaseDerivation`s. This theorem shows how this would look. -/
-theorem predecessor_iff {N : Type u} [ChaseNode N obs rules] {cd : ChaseDerivation N obs rules} (n1 n2 : Node cd) :
+theorem predecessor_iff {cd : ChaseDerivation N obs rules} (n1 n2 : Node cd) :
     n1 ≼ n2 ↔ ∃ cd2, cd2 <:+ cd ∧ cd2.head = n1.val ∧ n2.val ∈ cd2 := by
   constructor
   . rintro ⟨cds2, suf, head, mem⟩; exists cd.derivation_for_skeleton cds2 suf
   . rintro ⟨cd2, suf, head, mem⟩; exists cd2.toChaseDerivationSkeleton
 
-/-- The predecessor relation is antisymmetric. -/
-@[grind ->]
-theorem predecessor_antisymm {cd : ChaseDerivation (RegularChaseNode obs rules) obs rules} {n1 n2 : Node cd} : n1 ≼ n2 -> n2 ≼ n1 -> n1 = n2 := by
-  simp only [predecessor_iff]; grind
-
-/-- The predecessor relation is transitive. -/
-@[grind ->]
-theorem predecessor_trans {cd : ChaseDerivation (RegularChaseNode obs rules) obs rules} {n1 n2 n3 : Node cd} : n1 ≼ n2 -> n2 ≼ n3 -> n1 ≼ n3 := by
-  simp only [predecessor_iff]; grind
-
-/-- We can express fairness in terms of the predecessor relation: For each trigger, there is a node such that the trigger is not active for each of the node's successors. -/
-theorem fairness_prec {cd : ChaseDerivation (RegularChaseNode obs rules) obs rules} : ∀ (trg : RTrigger obs rules), ∃ (node : cd.Node), ∀ node2, node ≼ node2 -> ¬ trg.val.active node2.val.facts := by
-  intro trg
-  rcases cd.fairness' trg with ⟨cd2, suffix, fair⟩
-  exists ⟨cd2.head, cd2.mem_of_mem_suffix suffix _ cd2.head_mem⟩
-  intro node2 prec
-  apply fair
-  rw [predecessor_iff] at prec
-  rcases prec with ⟨cd3, suf3, head3, node2_mem_cd3⟩
-  simp only at head3
-  have : cd3 = cd2 := by
-    have : cd2.head ∈ cd2 := cd2.head_mem
-    apply eq_of_suffix_of_head_mem _ (by rw [← head3]; exact cd3.head_mem)
-    apply suffix_of_suffix_of_suffix_of_head_mem suffix suf3
-    rw [head3]; exact cd2.head_mem
-  rw [← this]
-  exact node2_mem_cd3
-
-section StrictPredecessor
-
-/-!
-The strict version of the predecessor is a strict total order on `ChaseDerivation.Node` for the `ChaseDerivation`.
--/
-
-/-- The strict predecessor relation is asymmetric. -/
-@[grind ->]
-theorem strict_predecessor_asymmetric {cd : ChaseDerivation (RegularChaseNode obs rules) obs rules} {n1 n2 : Node cd} : n1 ≺ n2 -> ¬ n2 ≺ n1 := by
-  intro prec contra; apply prec.right; apply predecessor_antisymm prec.left contra.left
-
-/-- The strict predecessor relation is transitive. -/
-@[grind ->]
-theorem strict_predecessor_trans {cd : ChaseDerivation (RegularChaseNode obs rules) obs rules} {n1 n2 n3 : Node cd} : n1 ≺ n2 -> n2 ≺ n3 -> n1 ≺ n3 := by
-  intro prec1 prec2
-  constructor
-  . exact predecessor_trans prec1.left prec2.left
-  . grind
-
-/-- The `ChaseDerivationSkeleton.head` is a strict predecessor of `ChaseDerivationSkeleton.next`. -/
-theorem head_strict_prec_next {cd : ChaseDerivation (RegularChaseNode obs rules) obs rules} :
-    ∀ {next}, (mem : next ∈ cd.next) -> ⟨cd.head, cd.head_mem⟩ ≺ ⟨next, cd.next_mem_of_mem _ mem⟩ := by
-  intro next next_mem
-  constructor
-  . exact cd.head_prec_next next_mem
-  . intro contra
-    apply cd.head_not_mem_tail (by rw [next_mem]; simp)
-    grind
-
-/-- The facts of a strict successor cannot be a subset of our facts. This is because strict successor nodes can only be introduced by active triggers. But if a trigger only produces facts that already exist, then it cannot be active. -/
-@[grind ->]
-theorem facts_not_subset_of_strict_predecessor {cd : ChaseDerivation (RegularChaseNode obs rules) obs rules} {n1 n2 : Node cd} :
-    n1 ≺ n2 -> ¬ n2.val.facts ⊆ n1.val.facts := by
-  intro prec contra
-  rcases (predecessor_iff _ _).mp prec.left with ⟨d, suf, head, mem⟩
-  rcases cd.subderivation_of_node_mem n2.property with ⟨d2, head2, suf2⟩
-  have suf3 : d2 <:+ d := suffix_of_suffix_of_suffix_of_head_mem suf suf2 (by rw [head2]; exact mem)
-  cases ChaseDerivation.suffix_iff_eq_or_suffix_tail.mp suf3 with
-  | inl suf3 => grind
-  | inr suf3 =>
-    rcases suf3 with ⟨next_some, suf3⟩
-    rw [Option.isSome_iff_exists] at next_some
-    rcases next_some with ⟨next, next_some⟩
-    apply (d.active_trigger_origin_next next_some).right
-    apply ObsolescenceCondition.contains_trg_result_implies_cond
-    have : next.facts ⊆ d.head.facts := by
-      have : ⟨next, d.next_mem_of_mem _ next_some⟩ ≼ ⟨n2.val, by apply ChaseDerivation.mem_of_mem_suffix (d2.branch.IsSuffix_trans suf3 d.branch.IsSuffix_tail); rw [← head2]; exact d2.head_mem⟩ := by
-        rw [predecessor_iff]
-        exists d.tail (by simp [next_some])
-        constructor
-        . exact PossiblyInfiniteList.IsSuffix_tail
-        constructor
-        . simp [d.head_tail', next_some]
-        . apply ChaseDerivation.mem_of_mem_suffix suf3; rw [← head2]; exact d2.head_mem
-      grind
-    exact Set.subset_trans (by rw [← next.ingoingFacts_eq, d.facts_next next_some]; apply Set.subset_union_of_subset_right; apply Set.subset_refl) this
-
-end StrictPredecessor
-
 end Predecessors
-
-public section ChaseResult
-
-/-!
-## Chase Result
-
-Opposed to the `ChaseDerivationSkeleton`, the result is now a model for all rules.
--/
-
-/-- The result is a model of all rules. This is true because otherwise, there would be an active trigger on the result. But then, this trigger needs to be active for some node and the hence it needs to become inactive at some point due to fairness. Hence it cannot be active on the result. Contradiction! -/
-@[grind <-]
-theorem result_models_rules {cd : ChaseDerivation (RegularChaseNode obs rules) obs rules} : cd.result.modelsRules rules := by
-  intro r r_mem subs subs_loaded
-  let trg : Trigger obs := ⟨r, subs⟩
-  have trg_loaded : trg.loaded cd.result := subs_loaded
-  apply obs.cond_implies_trg_is_satisfied (trg := trg)
-  rcases cd.trg_loaded_for_some_node_of_trg_loaded_for_result trg trg_loaded with ⟨node_loaded, node_loaded_mem, trg_loaded⟩
-  rcases cd.subderivation_of_node_mem node_loaded_mem with ⟨cd_loaded, cd_loaded_head, cd_loaded_suffix⟩
-  rcases cd_loaded.fairness' ⟨trg, r_mem⟩ with ⟨cd_obs, cd_obs_suffix, fairness⟩
-  specialize fairness cd_obs.head cd_obs.head_mem
-  apply Classical.byContradiction
-  intro contra_not_obs
-  apply fairness
-  constructor
-  . apply Set.subset_trans trg_loaded
-    rw [← cd_loaded_head]
-    apply cd_loaded.facts_node_subset_every_mem
-    apply cd_obs.mem_of_mem_suffix cd_obs_suffix
-    apply cd_obs.head_mem
-  . intro contra
-    apply contra_not_obs
-    rw [← ChaseDerivationSkeleton.result_suffix (PossiblyInfiniteList.IsSuffix_trans cd_obs_suffix cd_loaded_suffix)]
-    apply obs.monotone
-    . apply cd_obs.facts_node_subset_result; apply cd_obs.head_mem
-    . exact contra
-
-end ChaseResult
 
 public section TermsInChase
 
@@ -488,24 +317,30 @@ The second observation entails that the precense of a functional term that does 
 that the trigger that introduces this term must have been applied in some `ChaseNode`.
 -/
 
+variable {N : Type u} [CN : ChaseNode N obs rules]
+
 /-- Constants in the chase can only come from the initial fact set or from a constant in a rule. -/
 theorem constants_node_subset_constants_fs_union_constants_rules
-    {cd : ChaseDerivation (RegularChaseNode obs rules) obs rules} {node : RegularChaseNode obs rules} (node_mem : node ∈ cd) :
-    node.facts.constants ⊆ (cd.head.facts.constants ∪ rules.head_constants) := by
+    (out_sub_in : CN.out_sub_in)
+    {cd : ChaseDerivation N obs rules}
+    (start_eq : CN.ingoingFacts cd.head = CN.outgoingFacts cd.head)
+    {node : N} (node_mem : node ∈ cd) :
+    (CN.ingoingFacts node).constants ⊆ ((CN.outgoingFacts cd.head).constants ∪ rules.head_constants) := by
   let node' : cd.Node := ⟨node, node_mem⟩
-  show node'.val.facts.constants ⊆ (cd.head.facts.constants ∪ rules.head_constants)
+  show (CN.ingoingFacts node'.val).constants ⊆ ((CN.outgoingFacts cd.head).constants ∪ rules.head_constants)
   induction node' using mem_rec with
   | head =>
     apply Set.subset_union_of_subset_left
+    rw [start_eq]
     apply Set.subset_refl
   | step cd2 suffix ih next next_eq =>
-    rw [← next.ingoingFacts_eq, ChaseDerivationSkeleton.facts_next next_eq]
+    rw [ChaseDerivationSkeleton.facts_next next_eq]
     intro c c_mem
     rw [FactSet.constants_union] at c_mem
     cases c_mem with
-    | inl c_mem => apply ih; exact c_mem
+    | inl c_mem => apply ih; apply FactSet.constants_subset_of_subset out_sub_in; exact c_mem
     | inr c_mem =>
-      let origin := next.origin.get (cd2.isSome_origin_next next_eq)
+      let origin := (CN.origin next).get (cd2.isSome_origin_next next_eq)
       apply Set.subset_trans (origin.fst.val.mapped_head_constants_subset origin.snd)
       . intro c c_mem
         rw [List.mem_toSet, List.mem_append] at c_mem
@@ -519,7 +354,8 @@ theorem constants_node_subset_constants_fs_union_constants_rules
           rcases FunctionFreeConjunction.mem_vars.mp (origin.fst.val.rule.frontier_subset_vars_body v_mem) with ⟨a, a_mem, v_mem'⟩
           exists origin.fst.val.subs.apply_function_free_atom a
           constructor
-          . apply (cd2.active_trigger_origin_next next_eq).left
+          . apply out_sub_in
+            apply (cd2.active_trigger_origin_next next_eq).left
             rw [List.mem_toSet]
             apply TermMapping.apply_generalized_atom_mem_apply_generalized_atom_list
             exact a_mem
@@ -548,18 +384,21 @@ theorem constants_node_subset_constants_fs_union_constants_rules
 
 /-- Each functional term in the chase originates as a fresh term from a trigger if it was not already part of the initial fact set. -/
 theorem functional_term_originates_from_some_trigger
-    {cd : ChaseDerivation (RegularChaseNode obs rules) obs rules}
+    (out_sub_in : CN.out_sub_in)
+    {cd : ChaseDerivation N obs rules}
+    (start_eq : CN.ingoingFacts cd.head = CN.outgoingFacts cd.head)
+    (predecessor_trans : ∀ {n1 n2 n3 : cd.Node}, n1 ≼ n2 -> n2 ≼ n3 -> n1 ≼ n3)
     (node : Node cd)
     {t : GroundTerm sig}
     (t_is_func : ∃ func ts arity_ok, t = GroundTerm.func func ts arity_ok)
-    (t_mem : t ∈ node.val.facts.terms) :
-    t ∈ cd.head.facts.terms ∨ ∃ node2, node2 ≼ node ∧ ∃ orig ∈ node2.val.origin, t ∈ orig.fst.val.fresh_terms_for_head_disjunct orig.snd.val (by rw [← PreTrigger.length_mapped_head]; exact orig.snd.isLt) := by
+    (t_mem : t ∈ (CN.ingoingFacts node.val).terms) :
+    t ∈ (CN.outgoingFacts cd.head).terms ∨ ∃ node2, node2 ≼ node ∧ ∃ orig ∈ (CN.origin node2.val), t ∈ orig.fst.val.fresh_terms_for_head_disjunct orig.snd.val (by rw [← PreTrigger.length_mapped_head]; exact orig.snd.isLt) := by
   induction node using mem_rec with
-  | head => apply Or.inl; exact t_mem
+  | head => apply Or.inl; rw [← start_eq]; exact t_mem
   | step cd2 suffix ih next next_mem =>
-    rw [← next.ingoingFacts_eq, cd2.facts_next next_mem, FactSet.terms_union] at t_mem
+    rw [cd2.facts_next next_mem, FactSet.terms_union] at t_mem
 
-    have aux : t ∈ cd2.head.facts.terms -> t ∈ cd.head.facts.terms ∨ ∃ (node2 : cd.Node), node2 ≼ ⟨next, cd2.mem_of_mem_suffix suffix _ (cd2.next_mem_of_mem _ next_mem)⟩ ∧ ∃ orig ∈ node2.val.origin, t ∈ orig.fst.val.fresh_terms_for_head_disjunct orig.snd.val (by rw [← PreTrigger.length_mapped_head]; exact orig.snd.isLt) := by
+    have aux : t ∈ (CN.ingoingFacts cd2.head).terms -> t ∈ (CN.outgoingFacts cd.head).terms ∨ ∃ (node2 : cd.Node), node2 ≼ ⟨next, cd2.mem_of_mem_suffix suffix _ (cd2.next_mem_of_mem _ next_mem)⟩ ∧ ∃ orig ∈ (CN.origin node2.val), t ∈ orig.fst.val.fresh_terms_for_head_disjunct orig.snd.val (by rw [← PreTrigger.length_mapped_head]; exact orig.snd.isLt) := by
       intro t_mem
       cases ih t_mem with
       | inl ih => apply Or.inl; exact ih
@@ -571,7 +410,7 @@ theorem functional_term_originates_from_some_trigger
         . exact t_mem
 
     cases t_mem with
-    | inl t_mem => exact aux t_mem
+    | inl t_mem => exact aux (FactSet.terms_subset_of_subset out_sub_in _ t_mem)
     | inr t_mem =>
       unfold ChaseNode.origin_result at t_mem
       rw [FactSet.mem_terms_toSet, PreTrigger.mem_terms_mapped_head_iff] at t_mem
@@ -582,11 +421,12 @@ theorem functional_term_originates_from_some_trigger
       | inr t_mem =>
         apply Or.inr; exists ⟨next, cd2.mem_of_mem_suffix suffix _ (cd2.next_mem_of_mem _ next_mem)⟩; constructor
         . exact ChaseDerivationSkeleton.predecessor_refl
-        . exists next.origin.get (cd2.isSome_origin_next next_mem)
+        . exists (CN.origin next).get (cd2.isSome_origin_next next_mem)
           simp only [Option.get_mem, true_and]
           exact t_mem
       | inl t_mem =>
         apply aux
+        apply FactSet.terms_subset_of_subset out_sub_in
         apply FactSet.terms_subset_of_subset (cd2.active_trigger_origin_next next_mem).left
         rw [List.mem_map] at t_mem
         rcases t_mem with ⟨v, v_mem, t_mem⟩
@@ -597,16 +437,19 @@ theorem functional_term_originates_from_some_trigger
 
 /-- If a functional term occurs in the chase, then the trigger that introduces this term must have been used in the chase, unless the term already occurs in the initial fact set. -/
 theorem trigger_introducing_functional_term_occurs_in_chase
-    {cd : ChaseDerivation (RegularChaseNode obs rules) obs rules}
+    (out_sub_in : CN.out_sub_in)
+    {cd : ChaseDerivation N obs rules}
+    (start_eq : CN.ingoingFacts cd.head = CN.outgoingFacts cd.head)
+    (predecessor_trans : ∀ {n1 n2 n3 : cd.Node}, n1 ≼ n2 -> n2 ≼ n3 -> n1 ≼ n3)
     (node : Node cd)
     {t : GroundTerm sig}
-    (t_mem_node : t ∈ node.val.facts.terms)
+    (t_mem_node : t ∈ (CN.ingoingFacts node.val).terms)
     {trg : RTrigger obs rules}
     {disj_idx : Nat}
     {lt : disj_idx < trg.val.rule.head.length}
     (t_mem_trg : t ∈ trg.val.fresh_terms_for_head_disjunct disj_idx lt) :
-    t ∈ cd.head.facts.terms ∨ ∃ node2, node2 ≼ node ∧ ∃ orig ∈ node2.val.origin, orig.fst.equiv trg ∧ orig.snd.val = disj_idx := by
-  cases functional_term_originates_from_some_trigger node (by
+    t ∈ (CN.outgoingFacts cd.head).terms ∨ ∃ node2, node2 ≼ node ∧ ∃ orig ∈ (CN.origin node2.val), orig.fst.equiv trg ∧ orig.snd.val = disj_idx := by
+  cases functional_term_originates_from_some_trigger out_sub_in start_eq predecessor_trans node (by
     cases eq : t with
     | const _ =>
       rw [eq] at t_mem_trg
@@ -621,10 +464,258 @@ theorem trigger_introducing_functional_term_occurs_in_chase
     exists origin; simp only [origin_eq, true_and]
     exact RTrigger.equiv_of_term_mem_fresh_terms_for_head_disjunct t_mem t_mem_trg
 
+end TermsInChase
+
+end ChaseDerivation
+
+
+public abbrev RegularChaseDerivation (obs : ObsolescenceCondition sig) (rules : RuleSet sig) := ChaseDerivation (RegularChaseNode obs rules) obs rules
+
+namespace RegularChaseDerivation
+
+variable {obs : ObsolescenceCondition sig} {rules : RuleSet sig}
+
+public section FactMonotonicity
+
+/-!
+## Subset Monotonicity of Facts in ChaseNodes
+
+Compared to `ChaseDerivationSkeleton`, we get a couple of nice implications out of the subset monotonicity of fact sets. For example, we can never see the same `ChaseNode` twice as otherwise the trigger in second occurrence would already be obsolete.
+-/
+
+/-- Each member's facts contain the head facts. Note that this extends to arbitrary pairs of members since each member always induces a subderivation where it acts as the head. -/
+@[grind <-]
+theorem facts_node_subset_every_mem {cd : RegularChaseDerivation obs rules} : ∀ node ∈ cd, cd.head.facts ⊆ node.facts :=
+  RegularChaseDerivationSkeleton.facts_node_subset_every_mem
+
+/-- A first implication of `facts_node_subset_every_mem` is that, considering one of our subderivations, each of our members either has all of its facts contained in the head of the subderivation or it is itself a member of the subderivation. -/
+theorem mem_suffix_of_mem {cd1 cd2 : RegularChaseDerivation obs rules} (suffix : cd1 <:+ cd2) : ∀ node ∈ cd2, node.facts ⊆ cd1.head.facts ∨ node ∈ cd1 :=
+  RegularChaseDerivationSkeleton.mem_suffix_of_mem suffix
+
+/-- The `head` cannot occur in the `tail`. Otherwise, it would be introduced using a trigger but then this trigger is already obsolete since all the facts from `head` already occur in the very beginning. We use `ObsolescenceCondition.contains_trg_result_implies_cond` here. -/
+theorem head_not_mem_tail {cd : RegularChaseDerivation obs rules} : ∀ h, ¬ cd.head ∈ cd.tail h := by
+  intro h contra
+  rw [cd.mem_tail_iff] at contra
+  rcases contra with ⟨cd2, suffix, contra⟩
+  apply (cd2.active_trigger_origin_next contra).right
+  apply obs.contains_trg_result_implies_cond
+  apply Set.subset_trans (cd.head.facts_contain_origin_result (cd.head.origin.get (cd2.isSome_origin_next contra)) (by simp))
+  apply cd.facts_node_subset_every_mem
+  apply cd2.mem_of_mem_suffix suffix
+  exact cd2.head_mem
+
+/-- By `head_not_mem_tail`, if we have a suffix but our head occurs in the suffix, then our suffix is equal to us. -/
+@[grind ->]
+theorem eq_of_suffix_of_head_mem {cd1 cd2 : RegularChaseDerivation obs rules} (suffix : cd1 <:+ cd2) (head_mem : cd2.head ∈ cd1) : cd1 = cd2 := by
+  rw [ChaseDerivation.suffix_iff_eq_or_suffix_tail] at suffix
+  cases suffix with
+  | inl suffix => exact suffix
+  | inr suffix => rcases suffix with ⟨h, suffix⟩; apply False.elim; apply head_not_mem_tail h; apply cd1.mem_of_mem_suffix suffix; exact head_mem
+
+/-- And now by `eq_of_suffix_of_head_mem`, if we have two suffixes $C$ and $D$, and the head of $D$ occurs in $C$, then $D$ is a suffix of $C$. This may seem obvious even without the above results but it is really not even though it aligns well with one's intuition. Imagine that a `ChaseNode` could occur multiple times in a `ChaseDerivation`. Then we may have a case where $C$ is a subderivation of $D$, $D$ is not a subderivation of $C$ but $D$ occurs in $C$. -/
+@[grind ->]
+theorem suffix_of_suffix_of_suffix_of_head_mem {cd cd1 cd2 : RegularChaseDerivation obs rules} :
+    cd1 <:+ cd -> cd2 <:+ cd -> cd2.head ∈ cd1 -> cd2 <:+ cd1 := by
+  intro suffix1 suffix2 head_mem
+  cases PossiblyInfiniteList.suffix_or_suffix_of_suffix suffix1 suffix2 with
+  | inr suffix => exact suffix
+  | inl suffix => rw [eq_of_suffix_of_head_mem suffix]; exact PossiblyInfiniteList.IsSuffix_refl; exact head_mem
+
+end FactMonotonicity
+
+public section Predecessors
+
+/-!
+## Predecessor Relation
+
+Since we learned that `ChaseNode`s cannot occur multiple times in the same `ChaseDerivation`,
+the predecessor relation defined on `ChaseDerivationSkeleton` is now a total order on `ChaseDerivation.Node`.
+This is particularly nice, since we can do this while completely ignoring indices of the nodes in the underlying `PossiblyInfiniteList`.
+-/
+
+/-- The predecessor relation is antisymmetric. -/
+@[grind ->]
+theorem predecessor_antisymm {cd : RegularChaseDerivation obs rules} {n1 n2 : cd.Node} : n1 ≼ n2 -> n2 ≼ n1 -> n1 = n2 := by
+  simp only [cd.predecessor_iff]; grind
+
+/-- The predecessor relation is transitive. -/
+@[grind ->]
+theorem predecessor_trans {cd : RegularChaseDerivation obs rules} {n1 n2 n3 : cd.Node} : n1 ≼ n2 -> n2 ≼ n3 -> n1 ≼ n3 := by
+  simp only [cd.predecessor_iff]; grind
+
+/-- We can express fairness in terms of the predecessor relation: For each trigger, there is a node such that the trigger is not active for each of the node's successors. -/
+theorem fairness_prec {cd : RegularChaseDerivation obs rules} :
+    ∀ (trg : RTrigger obs rules), ∃ (node : cd.Node), ∀ node2, node ≼ node2 -> ¬ trg.val.active node2.val.facts := by
+  intro trg
+  rcases cd.fairness' trg with ⟨cd2, suffix, fair⟩
+  exists ⟨cd2.head, cd2.mem_of_mem_suffix suffix _ cd2.head_mem⟩
+  intro node2 prec
+  apply fair
+  rw [cd.predecessor_iff] at prec
+  rcases prec with ⟨cd3, suf3, head3, node2_mem_cd3⟩
+  simp only at head3
+  have : cd3 = cd2 := by
+    have : cd2.head ∈ cd2 := cd2.head_mem
+    apply eq_of_suffix_of_head_mem _ (by rw [← head3]; exact cd3.head_mem)
+    apply suffix_of_suffix_of_suffix_of_head_mem suffix suf3
+    rw [head3]; exact cd2.head_mem
+  rw [← this]
+  exact node2_mem_cd3
+
+section StrictPredecessor
+
+/-!
+The strict version of the predecessor is a strict total order on `ChaseDerivation.Node` for the `ChaseDerivation`.
+-/
+
+/-- The strict predecessor relation is asymmetric. -/
+@[grind ->]
+theorem strict_predecessor_asymmetric {cd : RegularChaseDerivation obs rules} {n1 n2 : cd.Node} : n1 ≺ n2 -> ¬ n2 ≺ n1 := by
+  intro prec contra; apply prec.right; apply predecessor_antisymm prec.left contra.left
+
+/-- The strict predecessor relation is transitive. -/
+@[grind ->]
+theorem strict_predecessor_trans {cd : RegularChaseDerivation obs rules} {n1 n2 n3 : cd.Node} : n1 ≺ n2 -> n2 ≺ n3 -> n1 ≺ n3 := by
+  intro prec1 prec2
+  constructor
+  . exact predecessor_trans prec1.left prec2.left
+  . grind
+
+/-- The `ChaseDerivationSkeleton.head` is a strict predecessor of `ChaseDerivationSkeleton.next`. -/
+theorem head_strict_prec_next {cd : RegularChaseDerivation obs rules} :
+    ∀ {next}, (mem : next ∈ cd.next) -> ⟨cd.head, cd.head_mem⟩ ≺ ⟨next, cd.next_mem_of_mem _ mem⟩ := by
+  intro next next_mem
+  constructor
+  . exact cd.head_prec_next next_mem
+  . intro contra
+    apply cd.head_not_mem_tail (by rw [next_mem]; simp)
+    grind
+
+/-- The facts of a strict successor cannot be a subset of our facts. This is because strict successor nodes can only be introduced by active triggers. But if a trigger only produces facts that already exist, then it cannot be active. -/
+@[grind ->]
+theorem facts_not_subset_of_strict_predecessor {cd : RegularChaseDerivation obs rules} {n1 n2 : cd.Node} :
+    n1 ≺ n2 -> ¬ n2.val.facts ⊆ n1.val.facts := by
+  intro prec contra
+  rcases (cd.predecessor_iff _ _).mp prec.left with ⟨d, suf, head, mem⟩
+  rcases cd.subderivation_of_node_mem n2.property with ⟨d2, head2, suf2⟩
+  have suf3 : d2 <:+ d := suffix_of_suffix_of_suffix_of_head_mem suf suf2 (by rw [head2]; exact mem)
+  cases ChaseDerivation.suffix_iff_eq_or_suffix_tail.mp suf3 with
+  | inl suf3 => grind
+  | inr suf3 =>
+    rcases suf3 with ⟨next_some, suf3⟩
+    rw [Option.isSome_iff_exists] at next_some
+    rcases next_some with ⟨next, next_some⟩
+    apply (d.active_trigger_origin_next next_some).right
+    apply ObsolescenceCondition.contains_trg_result_implies_cond
+    have : next.facts ⊆ d.head.facts := by
+      have : ⟨next, d.next_mem_of_mem _ next_some⟩ ≼ ⟨n2.val, by apply ChaseDerivation.mem_of_mem_suffix (d2.branch.IsSuffix_trans suf3 d.branch.IsSuffix_tail); rw [← head2]; exact d2.head_mem⟩ := by
+        rw [d.predecessor_iff]
+        exists d.tail (by simp [next_some])
+        constructor
+        . exact PossiblyInfiniteList.IsSuffix_tail
+        constructor
+        . simp [d.head_tail', next_some]
+        . apply ChaseDerivation.mem_of_mem_suffix suf3; rw [← head2]; exact d2.head_mem
+      grind
+    exact Set.subset_trans (by rw [← next.ingoingFacts_eq, d.facts_next next_some]; apply Set.subset_union_of_subset_right; apply Set.subset_refl) this
+
+end StrictPredecessor
+
+end Predecessors
+
+public section ChaseResult
+
+/-!
+## Chase Result
+
+Opposed to the `ChaseDerivationSkeleton`, the result is now a model for all rules.
+-/
+
+/-- We define a shortcut for `RegularChaseDerivationSkeleton.result`. -/
+abbrev result (cd : RegularChaseDerivation obs rules) := RegularChaseDerivationSkeleton.result cd.toChaseDerivationSkeleton
+
+/-- The result is a model of all rules. This is true because otherwise, there would be an active trigger on the result. But then, this trigger needs to be active for some node and the hence it needs to become inactive at some point due to fairness. Hence it cannot be active on the result. Contradiction! -/
+@[grind <-]
+theorem result_models_rules {cd : RegularChaseDerivation obs rules} : cd.result.modelsRules rules := by
+  intro r r_mem subs subs_loaded
+  let trg : Trigger obs := ⟨r, subs⟩
+  have trg_loaded : trg.loaded cd.result := subs_loaded
+  apply obs.cond_implies_trg_is_satisfied (trg := trg)
+  rcases RegularChaseDerivationSkeleton.trg_loaded_for_some_node_of_trg_loaded_for_result trg trg_loaded with ⟨node_loaded, node_loaded_mem, trg_loaded⟩
+  rcases cd.subderivation_of_node_mem node_loaded_mem with ⟨cd_loaded, cd_loaded_head, cd_loaded_suffix⟩
+  rcases cd_loaded.fairness' ⟨trg, r_mem⟩ with ⟨cd_obs, cd_obs_suffix, fairness⟩
+  specialize fairness cd_obs.head cd_obs.head_mem
+  apply Classical.byContradiction
+  intro contra_not_obs
+  apply fairness
+  constructor
+  . apply Set.subset_trans trg_loaded
+    rw [← cd_loaded_head]
+    apply RegularChaseDerivationSkeleton.facts_node_subset_every_mem
+    apply cd_obs.mem_of_mem_suffix cd_obs_suffix
+    apply cd_obs.head_mem
+  . intro contra
+    apply contra_not_obs
+    unfold result
+    rw [← RegularChaseDerivationSkeleton.result_suffix (PossiblyInfiniteList.IsSuffix_trans cd_obs_suffix cd_loaded_suffix)]
+    apply obs.monotone
+    . apply RegularChaseDerivationSkeleton.facts_node_subset_result; apply cd_obs.head_mem
+    . exact contra
+
+end ChaseResult
+
+public section TermsInChase
+
+/-!
+## Terms in the Chase
+
+We make some general observations about certain terms that might occur in the chase.
+
+1. Constants can only originate directly from rules or from the initial fact set. No other constants can be introduced.
+2. Functional terms can either also originate from the initial fact set or they are introduced as fresh terms by a trigger.
+
+The second observation entails that the precense of a functional term that does not occur in the initial fact set implies
+that the trigger that introduces this term must have been applied in some `ChaseNode`.
+-/
+
+
+/-- Constants in the chase can only come from the initial fact set or from a constant in a rule. -/
+theorem constants_node_subset_constants_fs_union_constants_rules
+    {cd : RegularChaseDerivation obs rules}
+    {node : RegularChaseNode obs rules} (node_mem : node ∈ cd) :
+    node.facts.constants ⊆ cd.head.facts.constants ∪ rules.head_constants := by
+  apply ChaseDerivation.constants_node_subset_constants_fs_union_constants_rules RegularChaseNode.out_sub_in _ node_mem
+  rw [RegularChaseNode.ingoingFacts_eq, RegularChaseNode.outgoingFacts_eq]
+
+/-- Each functional term in the chase originates as a fresh term from a trigger if it was not already part of the initial fact set. -/
+theorem functional_term_originates_from_some_trigger
+    {cd : RegularChaseDerivation obs rules}
+    (node : cd.Node)
+    {t : GroundTerm sig}
+    (t_is_func : ∃ func ts arity_ok, t = GroundTerm.func func ts arity_ok)
+    (t_mem : t ∈ node.val.facts.terms) :
+    t ∈ cd.head.facts.terms ∨ ∃ node2, node2 ≼ node ∧ ∃ orig ∈ node2.val.origin, t ∈ orig.fst.val.fresh_terms_for_head_disjunct orig.snd.val (by rw [← PreTrigger.length_mapped_head]; exact orig.snd.isLt) := by
+  apply ChaseDerivation.functional_term_originates_from_some_trigger RegularChaseNode.out_sub_in _ predecessor_trans node t_is_func t_mem
+  rw [RegularChaseNode.ingoingFacts_eq, RegularChaseNode.outgoingFacts_eq]
+
+/-- If a functional term occurs in the chase, then the trigger that introduces this term must have been used in the chase, unless the term already occurs in the initial fact set. -/
+theorem trigger_introducing_functional_term_occurs_in_chase
+    {cd : RegularChaseDerivation obs rules}
+    (node : cd.Node)
+    {t : GroundTerm sig}
+    (t_mem_node : t ∈ node.val.facts.terms)
+    {trg : RTrigger obs rules}
+    {disj_idx : Nat}
+    {lt : disj_idx < trg.val.rule.head.length}
+    (t_mem_trg : t ∈ trg.val.fresh_terms_for_head_disjunct disj_idx lt) :
+    t ∈ cd.head.facts.terms ∨ ∃ node2, node2 ≼ node ∧ ∃ orig ∈ node2.val.origin, orig.fst.equiv trg ∧ orig.snd.val = disj_idx := by
+  apply ChaseDerivation.trigger_introducing_functional_term_occurs_in_chase RegularChaseNode.out_sub_in _ predecessor_trans node t_mem_node t_mem_trg
+  rw [RegularChaseNode.ingoingFacts_eq, RegularChaseNode.outgoingFacts_eq]
+
 /-- If a functional term occurs in the chase, then the result of the trigger that introduces this term is contained in the current node, unless the functional term already occurs in the initial fact set. -/
 theorem result_of_trigger_introducing_functional_term_occurs_in_chase
-    {cd : ChaseDerivation (RegularChaseNode obs rules) obs rules}
-    (node : Node cd)
+    {cd : RegularChaseDerivation obs rules}
+    (node : cd.Node)
     {t : GroundTerm sig}
     (t_mem_node : t ∈ node.val.facts.terms)
     {trg : RTrigger obs rules}
@@ -637,7 +728,7 @@ theorem result_of_trigger_introducing_functional_term_occurs_in_chase
   | inr t_mem =>
     apply Or.inr
     rcases t_mem with ⟨node2, prec, origin, origin_eq, equiv, index_eq⟩
-    apply Set.subset_trans _ (cd.facts_node_subset_of_prec prec)
+    apply Set.subset_trans _ (RegularChaseDerivationSkeleton.facts_node_subset_of_prec prec)
     simp only [← PreTrigger.result_eq_of_equiv equiv, ← index_eq]
     exact node2.val.facts_contain_origin_result _ origin_eq
 
@@ -653,7 +744,8 @@ The result itself is `prop_for_node_has_minimal_such_node` and is shown via `pro
 This forces us to take into account specific node indices and therefore requires auxiliary theorems, mainly `get?_branch_injective`, which is shown using `node_has_unique_position`.
 -/
 
-theorem node_has_unique_position (cd : ChaseDerivation (RegularChaseNode obs rules) obs rules) : ∀ node, ∀ i j, i < j -> cd.branch.get? i = some node -> cd.branch.get? j ≠ some node := by
+theorem node_has_unique_position (cd : RegularChaseDerivation obs rules) :
+    ∀ node, ∀ i j, i < j -> cd.branch.get? i = some node -> cd.branch.get? j ≠ some node := by
   intro node i j lt eq_i eq_j
   have le := Nat.le_pred_of_lt lt
   let cds2 := cd.derivation_for_branch_suffix (cd.branch.drop j.pred) (PossiblyInfiniteList.IsSuffix_drop j.pred) (by
@@ -665,14 +757,14 @@ theorem node_has_unique_position (cd : ChaseDerivation (RegularChaseNode obs rul
   )
   let cd2 := cd.derivation_for_skeleton cds2 (PossiblyInfiniteList.IsSuffix_drop j.pred)
   have next_eq : cd2.next = some node := by
-    simp only [ChaseDerivationSkeleton.next, cd2, derivation_for_skeleton, cds2, ChaseDerivationSkeleton.derivation_for_branch_suffix, PossiblyInfiniteList.tail_drop, PossiblyInfiniteList.head_drop]
+    simp only [ChaseDerivationSkeleton.next, cd2, ChaseDerivation.derivation_for_skeleton, cds2, ChaseDerivationSkeleton.derivation_for_branch_suffix, PossiblyInfiniteList.tail_drop, PossiblyInfiniteList.head_drop]
     rw [Nat.succ_pred (Nat.ne_zero_of_lt lt)]
     exact eq_j
   apply (cd2.active_trigger_origin_next next_eq).right
   apply obs.contains_trg_result_implies_cond
   have sub : node.facts ⊆ cd2.head.facts := by
     let node : cd.Node := ⟨node, by exists i⟩
-    let node2 : cd.Node := ⟨cd2.head, by exists j.pred; simp only [cd2, derivation_for_skeleton, cds2, ChaseDerivationSkeleton.derivation_for_branch_suffix, ChaseDerivationSkeleton.head, Option.some_get, PossiblyInfiniteList.head_drop]; rfl⟩
+    let node2 : cd.Node := ⟨cd2.head, by exists j.pred; simp only [cd2, ChaseDerivation.derivation_for_skeleton, cds2, ChaseDerivationSkeleton.derivation_for_branch_suffix, ChaseDerivationSkeleton.head, Option.some_get, PossiblyInfiniteList.head_drop]; rfl⟩
     have prec : node ≼ node2 := by
       exists cd.derivation_for_branch_suffix (cd.branch.drop i) (PossiblyInfiniteList.IsSuffix_drop i) (by simp [PossiblyInfiniteList.head_drop, eq_i])
       simp only [ChaseDerivationSkeleton.derivation_for_branch_suffix, ChaseDerivationSkeleton.head, PossiblyInfiniteList.head_drop]
@@ -683,10 +775,10 @@ theorem node_has_unique_position (cd : ChaseDerivation (RegularChaseNode obs rul
       exists j.pred - i
       simp only [cds2, ChaseDerivationSkeleton.derivation_for_branch_suffix]
       grind
-    exact cd.facts_node_subset_of_prec prec
+    exact RegularChaseDerivationSkeleton.facts_node_subset_of_prec prec
   exact Set.subset_trans (node.facts_contain_origin_result (node.origin.get (cd2.isSome_origin_next next_eq)) (by simp)) sub
 
-theorem get?_branch_injective (cd : ChaseDerivation (RegularChaseNode obs rules) obs rules) : ∀ node, ∀ i j, cd.branch.get? i = some node -> cd.branch.get? j = some node -> i = j := by
+theorem get?_branch_injective (cd : RegularChaseDerivation obs rules) : ∀ node, ∀ i j, cd.branch.get? i = some node -> cd.branch.get? j = some node -> i = j := by
   intro node i j eq_i eq_j
   apply Decidable.byContradiction
   intro ne
@@ -694,7 +786,7 @@ theorem get?_branch_injective (cd : ChaseDerivation (RegularChaseNode obs rules)
   | inl lt => exact cd.node_has_unique_position node i j lt eq_i eq_j
   | inr lt => exact cd.node_has_unique_position node j i lt eq_j eq_i
 
-public theorem prop_for_node_has_minimal_such_node {cd : ChaseDerivation (RegularChaseNode obs rules) obs rules} (prop : cd.Node -> Prop) :
+public theorem prop_for_node_has_minimal_such_node {cd : RegularChaseDerivation obs rules} (prop : cd.Node -> Prop) :
     ∀ n, prop n -> ∃ n2, prop n2 ∧ ∀ n3, n3 ≺ n2 -> ¬ prop n3 := by
   let prop' : Nat -> Prop := fun i => ∃ (e : RegularChaseNode obs rules) (mem : e ∈ cd.branch.get? i), prop ⟨e, by exists i⟩
   intro n prop_n
@@ -709,13 +801,13 @@ public theorem prop_for_node_has_minimal_such_node {cd : ChaseDerivation (Regula
     intro le; simp only [Nat.not_lt] at le
     apply strict_predecessor_asymmetric prec
     constructor
-    . rw [predecessor_iff]
+    . rw [cd.predecessor_iff]
       have n2_mem' : n2 ∈ cd := by exists k
       rcases cd.subderivation_of_node_mem n2_mem' with ⟨cd2, head2, suf2⟩
       exists cd2; simp only [suf2, head2, true_and]
-      rw [mem_iff]
+      rw [cd2.mem_iff]
       exists j - k
-      unfold IsSuffix at suf2; rw [ChaseDerivationSkeleton.IsSuffix_iff] at suf2; rcases suf2 with ⟨k', suf2⟩
+      unfold ChaseDerivation.IsSuffix at suf2; rw [ChaseDerivationSkeleton.IsSuffix_iff] at suf2; rcases suf2 with ⟨k', suf2⟩
       have : k' = k := by
         apply cd.get?_branch_injective n2
         . rw [← head2]
@@ -730,5 +822,5 @@ public theorem prop_for_node_has_minimal_such_node {cd : ChaseDerivation (Regula
 
 end MinimalNodeWithProp
 
-end ChaseDerivation
+end RegularChaseDerivation
 
