ExistentialRules/ChaseSequence/ChaseTree.lean
@@ -35,17 +35,18 @@ structure ChaseTree (N : Type u) (obs : ObsolescenceCondition sig) (kb : Knowled
 namespace ChaseTree
 
 variable {obs : ObsolescenceCondition sig} {kb : KnowledgeBase sig}
+variable {N : Type u} [CN : ChaseNode N obs kb.rules]
 
-instance {N : Type u} [CN : ChaseNode N obs kb.rules] : Membership N (ChaseTree N obs kb) where
+instance : Membership N (ChaseTree N obs kb) where
   mem td node := node ∈ td.tree
 
 /-- An element is a member of the tree iff it occurs at some address. -/
-theorem mem_iff {N : Type u} [CN : ChaseNode N obs kb.rules] {ct : ChaseTree N obs kb} :
+theorem mem_iff {ct : ChaseTree N obs kb} :
   ∀ {e}, e ∈ ct ↔ ∃ ns, ct.tree.get? ns = some e := TreeDerivation.mem_iff
 
 /-- We can convert `ChaseDerivation`s that are branches in the `ChaseTree` to `ChaseBranch`es. -/
 @[expose]
-def chaseBranch_for_branch {N : Type u} [CN : ChaseNode N obs kb.rules] {ct : ChaseTree N obs kb} {branch : ChaseDerivation N obs kb.rules} (branch_mem : branch ∈ ct.branches) : ChaseBranch N obs kb := {
+def chaseBranch_for_branch {ct : ChaseTree N obs kb} {branch : ChaseDerivation N obs kb.rules} (branch_mem : branch ∈ ct.branches) : ChaseBranch N obs kb := {
   branch := branch.branch
   isSome_head := branch.isSome_head
   triggers_exist := branch.triggers_exist
@@ -60,22 +61,14 @@ def chaseBranch_for_branch {N : Type u} [CN : ChaseNode N obs kb.rules] {ct : Ch
 }
 
 /-- We restate the `database_first` condition in terms of the `TreeDerivation` vocabulary. -/
-theorem database_first' {N : Type u} [CN : ChaseNode N obs kb.rules] {ct : ChaseTree N obs kb} :
+theorem database_first' {ct : ChaseTree N obs kb} :
     CN.ingoingFacts ct.root = kb.db.toFactSet ∧
     CN.outgoingFacts ct.root = kb.db.toFactSet ∧
     CN.origin ct.root = none := by
   apply ct.database_first; simp [TreeDerivation.root]
 
-/-- Opposed to a `TreeDerivation`, we know that each node in a `ChaseBranch` has a finite set of facts. This is because the database is finite and each trigger only adds finitely many new facts. -/
-theorem facts_finite_of_mem {ct : ChaseTree (RegularChaseNode obs kb.rules) obs kb} {node : RegularChaseNode obs kb.rules} (node_mem : node ∈ ct) :
-    node.facts.finite := by
-  rw [ct.facts_node_eq_union_initial_and_generated node_mem]
-  apply Set.union_finite_of_both_finite
-  . rw [← ct.root.outgoingFacts_eq, database_first'.right.left]; exact kb.db.toFactSet.property.left
-  . exact ct.generatedFacts_finite_of_mem node_mem
-
 /-- The root of the `ChaseTree` does not contain any function terms. -/
-theorem func_term_not_mem_root {N : Type u} [CN : ChaseNode N obs kb.rules] {ct : ChaseTree N obs kb}
+theorem func_term_not_mem_root {ct : ChaseTree N obs kb}
     {t : GroundTerm sig} (t_is_func : ∃ func ts arity_ok, t = GroundTerm.func func ts arity_ok) :
     ¬ t ∈ (CN.outgoingFacts ct.root).terms := by
   intro t_mem
@@ -86,38 +79,58 @@ theorem func_term_not_mem_root {N : Type u} [CN : ChaseNode N obs kb.rules] {ct 
   rw [t_eq'] at t_eq
   simp [GroundTerm.func_neq_const] at t_eq
 
+end ChaseTree
+
+
+abbrev RegularChaseTree (obs : ObsolescenceCondition sig) (kb : KnowledgeBase sig) := ChaseTree (RegularChaseNode obs kb.rules) obs kb
+
+namespace RegularChaseTree
+
+variable {obs : ObsolescenceCondition sig} {kb : KnowledgeBase sig}
+
+/-- Opposed to a `TreeDerivation`, we know that each node in a `ChaseBranch` has a finite set of facts. This is because the database is finite and each trigger only adds finitely many new facts. -/
+theorem facts_finite_of_mem {ct : RegularChaseTree obs kb} {node : RegularChaseNode obs kb.rules} (node_mem : node ∈ ct) :
+    node.facts.finite := by
+  rw [RegularTreeDerivation.facts_node_eq_union_initial_and_generated node_mem]
+  apply Set.union_finite_of_both_finite
+  . rw [← ct.root.outgoingFacts_eq, ct.database_first'.right.left]; exact kb.db.toFactSet.property.left
+  . exact RegularTreeDerivation.generatedFacts_finite_of_mem node_mem
+
+/-- We define a shortcut for `RegularTreeDerivation.result`. -/
+abbrev result (ct : RegularChaseTree obs kb) := RegularTreeDerivation.result ct.toTreeDerivation
+
 /-- Each element of the result of a `ChaseTree` not only models the rule set but the whole `KnowledgeBase`. -/
-theorem result_models_kb {ct : ChaseTree (RegularChaseNode obs kb.rules) obs kb} : ∀ fs ∈ ct.result, fs.modelsKb kb := by
-  unfold TreeDerivation.result; simp only [Set.mem_map]
+theorem result_models_kb {ct : RegularChaseTree obs kb} : ∀ fs ∈ ct.result, fs.modelsKb kb := by
+  unfold result RegularTreeDerivation.result; simp only [Set.mem_map]
   intro fs ⟨branch, branch_mem, fs_mem⟩
   let cb := ct.chaseBranch_for_branch branch_mem
-  have : branch.result = cb.result := by rfl
+  have : RegularChaseDerivationSkeleton.result branch.toChaseDerivationSkeleton = RegularChaseDerivationSkeleton.result cb.toChaseDerivationSkeleton := by rfl
   simp only [← fs_mem, this]
-  exact cb.result_models_kb
+  exact RegularChaseBranch.result_models_kb
 
 /-- Constants in the chase must be in the database or in some rule. -/
-theorem constants_node_subset_constants_db_union_constants_rules {ct : ChaseTree (RegularChaseNode obs kb.rules) obs kb}
+theorem constants_node_subset_constants_db_union_constants_rules {ct : RegularChaseTree obs kb}
     {node : RegularChaseNode obs kb.rules} (node_mem : node ∈ ct) :
     node.facts.constants ⊆ (kb.db.constants.val ∪ kb.rules.head_constants) := by
-  have := ct.constants_node_subset_constants_fs_union_constants_rules node_mem
+  have := RegularTreeDerivation.constants_node_subset_constants_fs_union_constants_rules node_mem
   rw [← ct.root.outgoingFacts_eq, ct.database_first'.right.left, Database.toFactSet_constants_same] at this
   exact this
 
 /-- Each functional term in the chase originates as a fresh term from a trigger. -/
 theorem functional_term_originates_from_some_trigger
-    {ct : ChaseTree (RegularChaseNode obs kb.rules) obs kb}
+    {ct : RegularChaseTree obs kb}
     (node : ct.NodeWithAddress)
     {t : GroundTerm sig}
     (t_is_func : ∃ func ts arity_ok, t = GroundTerm.func func ts arity_ok)
     (t_mem : t ∈ node.node.facts.terms) :
     ∃ node2, node2 ≼ node ∧ ∃ orig ∈ node2.node.origin, t ∈ orig.fst.val.fresh_terms_for_head_disjunct orig.snd.val (by grind) := by
-  cases TreeDerivation.functional_term_originates_from_some_trigger node t_is_func t_mem with
+  cases RegularTreeDerivation.functional_term_originates_from_some_trigger node t_is_func t_mem with
   | inl t_mem => apply False.elim; exact ct.func_term_not_mem_root t_is_func t_mem
   | inr t_mem => exact t_mem
 
 /-- If a functional term occurs in the chase, then the trigger that introduces this term must have been used in the chase. -/
 theorem trigger_introducing_functional_term_occurs_in_chase
-    {ct : ChaseTree (RegularChaseNode obs kb.rules) obs kb}
+    {ct : RegularChaseTree obs kb}
     (node : ct.NodeWithAddress)
     {t : GroundTerm sig}
     (t_mem_node : t ∈ node.node.facts.terms)
@@ -126,13 +139,13 @@ theorem trigger_introducing_functional_term_occurs_in_chase
     {lt : disj_idx < trg.val.rule.head.length}
     (t_mem_trg : t ∈ trg.val.fresh_terms_for_head_disjunct disj_idx lt) :
     ∃ node2, node2 ≼ node ∧ ∃ orig ∈ node2.node.origin, orig.fst.equiv trg ∧ orig.snd.val = disj_idx := by
-  cases TreeDerivation.trigger_introducing_functional_term_occurs_in_chase node t_mem_node t_mem_trg with
+  cases RegularTreeDerivation.trigger_introducing_functional_term_occurs_in_chase node t_mem_node t_mem_trg with
   | inl t_mem => apply False.elim; exact ct.func_term_not_mem_root (PreTrigger.term_functional_of_mem_fresh_terms _ t_mem_trg) t_mem
   | inr t_mem => exact t_mem
 
 /-- If a functional term occurs in the chase, then the result of the trigger that introduces this term is contained in the current node. -/
 theorem result_of_trigger_introducing_functional_term_occurs_in_chase
-    {ct : ChaseTree (RegularChaseNode obs kb.rules) obs kb}
+    {ct : RegularChaseTree obs kb}
     (node : ct.NodeWithAddress)
     {t : GroundTerm sig}
     (t_mem_node : t ∈ node.node.facts.terms)
@@ -140,9 +153,9 @@ theorem result_of_trigger_introducing_functional_term_occurs_in_chase
     {disj_idx : Nat}
     {lt : disj_idx < trg.val.rule.head.length}
     (t_mem_trg : t ∈ trg.val.fresh_terms_for_head_disjunct disj_idx lt) : (trg.val.mapped_head[disj_idx]'(by simpa)).toSet ⊆ node.node.facts := by
-  cases TreeDerivation.result_of_trigger_introducing_functional_term_occurs_in_chase node t_mem_node t_mem_trg with
+  cases RegularTreeDerivation.result_of_trigger_introducing_functional_term_occurs_in_chase node t_mem_node t_mem_trg with
   | inl t_mem => apply False.elim; exact ct.func_term_not_mem_root (PreTrigger.term_functional_of_mem_fresh_terms _ t_mem_trg) t_mem
   | inr t_mem => exact t_mem
 
-end ChaseTree
+end RegularChaseTree
 
